remove Function

Tactics/Coinc/ColR.v
@@ -197,17 +197,18 @@ apply exists_witness_ok with
 [intros x y HXY; apply proper_1; assumption|assumption].
 Qed.
 
-Function identify_lines (ss : (@TCSets.t SS)) (sp : (@TCSets.t SP))
-         {measure cardinal ss} : (@TCSets.t SS) :=
+Fixpoint identify_lines (ss : (@TCSets.t SS)) (sp : (@TCSets.t SP)) (n : nat) :
+  (@TCSets.t SS) :=
   let lines := pick_lines ss sp in
-    match lines with
-      | None         => ss
-      | Some (s1,s2) =>
+    match n, lines with
+      | Datatypes.S k, Some (s1,s2) =>
          let auxsetofsets := (@remove SS) s2 ((@remove SS) s1 ss) in
          let auxset := (@union S) s1 s2 in
          let newss := (@add SS) auxset auxsetofsets in
-         identify_lines newss sp
+         identify_lines newss sp k
+      | _            , _            => ss
     end.
+(*
 Proof.
 intros.
 assert (Datatypes.S(cardinal (remove s1 ss)) = cardinal ss)
@@ -237,9 +238,10 @@ elim ((@In_dec SS) (union s1 s2) (remove s2 (remove s1 ss))); intro HDec.
   rewrite HR2, <- HR1; apply le_n.
   }
 Defined.
+*)
 
 Definition test_col ss sp p1 p2 p3 : bool :=
-  let newss := identify_lines ss sp  in
+  let newss := identify_lines ss sp (cardinal ss)  in
     (@exists_ SS) (fun s => mem p1 s && mem p2 s && mem p3 s) newss.
 
 Section Col_refl.
@@ -299,36 +301,75 @@ Definition ss_ok (ss : (@TCSets.t SS)) (interp: positive -> COLTpoint) :=
 Definition sp_ok (sp : (@TCSets.t SP)) (interp: positive -> COLTpoint) :=
   forall p, mem p sp = true -> interp (fstpp p) <> interp (sndpp p).
 
+(*
+Lemma cardinal_newss1 : forall s1 s2 ss sp,
+  pick_lines ss sp = Some (s1,s2) ->
+  (@In SS) (union s1 s2) (@remove SS s2 (@remove SS s1 ss)) ->
+   Datatypes.S (Datatypes.S (cardinal
+                               (@add SS (union s1 s2)
+                                     (@remove SS s2 (@remove SS s1 ss))))) =
+   cardinal ss.
+Proof.
+intros s1 s2 ss sp Hs1s2 HIn; rewrite add_cardinal_1; [|auto].
+transitivity (Datatypes.S (cardinal (@remove SS s1 ss)));
+[apply eq_S|]; apply remove_cardinal_1;
+[apply pick_lines_ok_2 with sp|apply pick_lines_ok_1 with s2 sp]; auto.
+Qed.
+
+Lemma cardinal_newss2 : forall s1 s2 ss sp,
+  pick_lines ss sp = Some (s1,s2) ->
+  ~ (@In SS) (union s1 s2) (@remove SS s2 (@remove SS s1 ss)) ->
+   Datatypes.S (cardinal
+                  (@add SS (union s1 s2)
+                        (@remove SS s2 (@remove SS s1 ss)))) =
+   cardinal ss.
+Proof.
+intros s1 s2 ss sp Hs1s2 HIn; rewrite add_cardinal_2; [|auto].
+transitivity (Datatypes.S (cardinal (@remove SS s1 ss)));
+[apply eq_S|]; apply remove_cardinal_1;
+[apply pick_lines_ok_2 with sp|apply pick_lines_ok_1 with s2 sp]; auto.
+Qed.
+*)
+
+Lemma strong_induction : forall (P: nat -> Prop),
+  (forall m, (forall n, n < m -> P n) -> P m) ->
+  forall n, P n.
+Proof.
+intros P IH.
+assert (P0 : P 0) by (apply IH; intros m H; exfalso; inversion H).
+intros n; destruct n as [|n]; [auto|].
+cut (forall n, (forall m, m <= n -> P m)); [eauto|clear n].
+intro n; induction n; intros m Hm; inversion Hm; [auto| |eauto].
+subst; apply IH; intros; apply IHn; apply Gt.gt_S_le; auto.
+Qed.
+
 Lemma identify_lines_ok : forall ss sp interp,
   ss_ok ss interp -> sp_ok sp interp ->
-  ss_ok (identify_lines ss sp) interp.
+  ss_ok (identify_lines ss sp (cardinal ss)) interp.
 Proof.
-intros ss sp interp HSS HSP.
-apply (let P interp ss sp newss :=
-       ss_ok ss interp -> sp_ok sp interp -> ss_ok newss interp in
-         identify_lines_ind (P interp)); try assumption; [intros; assumption|].
-clear HSS; clear HSP; clear ss; clear sp.
-intros ss sp suitablepairofsets s1 s2 Hs1s2 auxsetofsets auxset newss H HSS HSP.
-assert (Hs1 := Hs1s2); assert (Hs2 := Hs1s2).
+intros ss.
+assert (Hn : exists n, cardinal ss = n) by (exists (cardinal ss); auto).
+destruct Hn as [n Hn]; rewrite Hn; clear Hn; revert ss.
+induction n  as [n IHn] using strong_induction.
+intros ss sp interp HSS HSP; simpl; destruct n; simpl; [auto|].
+assert (Hs1s2 : exists s1s2, pick_lines ss sp = s1s2);
+[exists (pick_lines ss sp); auto|destruct Hs1s2 as [p Hs1s2]].
+revert Hs1s2; elim p; [intros [s1 s2] Hs1s2|intro H; rewrite H; auto].
+rewrite Hs1s2; assert (Hs1 := Hs1s2); assert (Hs2 := Hs1s2).
 apply pick_lines_ok_1 in Hs1; apply pick_lines_ok_2 in Hs2.
-apply remove_3 in Hs2.
-apply H; try assumption; clear H.
-intros s Hmem p1 p2 p3 Hmemp.
+apply IHn; [auto|clear IHn p|auto].
+apply remove_3 in Hs2; intros s Hmem p1 p2 p3 Hmemp.
 do 2 (rewrite andb_true_iff in Hmemp).
 destruct Hmemp as [[Hmemp1 Hmemp2] Hmemp3].
-unfold newss in Hmem; clear newss.
-assert (HEq : Equal auxset s \/ ~ Equal auxset s)
-  by (rewrite <- equal_Equal; elim (equal auxset s); auto).
+assert (HEq : Equal (union s1 s2) s \/ ~ Equal (union s1 s2) s)
+  by (rewrite <- equal_Equal; elim (equal (union s1 s2) s); auto).
 destruct HEq as [HEq|HEq];
-[|rewrite add_neq_b in Hmem; try assumption;
- apply HSS with s; [|do 2 (rewrite andb_true_iff); repeat split; assumption];
- unfold auxsetofsets in *; apply mem_2 in Hmem;
- do 2 (apply remove_3 in Hmem); apply mem_1; assumption].
+[|rewrite add_neq_b in Hmem; [|auto]; apply HSS with s;
+  [apply mem_2, remove_3, remove_3, mem_1 in Hmem; auto|];
+  do 2 (rewrite andb_true_iff); repeat split; auto].
 rewrite <- ((@mem_m S) _ _ (TCSets.eq_refl p1) _ _ HEq) in Hmemp1.
 rewrite <- ((@mem_m S) _ _ (TCSets.eq_refl p2) _ _ HEq) in Hmemp2.
 rewrite <- ((@mem_m S) _ _ (TCSets.eq_refl p3) _ _ HEq) in Hmemp3.
-clear HEq; clear Hmem; clear s.
-unfold suitablepairofsets in Hs1s2; clear suitablepairofsets.
 unfold pick_lines in Hs1s2.
 case_eq (exists_witness
            (fun s : elt =>
@@ -357,11 +398,10 @@ apply HSP in HmemSP.
 apply mem_2 in Hmemfsts; apply mem_2 in Hmemsnds.
 apply inter_spec in Hmemfsts; destruct Hmemfsts as [Hfss1 Hfss2].
 apply inter_spec in Hmemsnds; destruct Hmemsnds as [Hsss1 Hsss2].
-unfold auxset in *.
 apply mem_2, union_1 in Hmemp1.
 apply mem_2, union_1 in Hmemp2.
 apply mem_2, union_1 in Hmemp3.
-apply CTcol3 with (interp (fstpp(x))) (interp (sndpp(x))); try assumption.
+apply CTcol3 with (interp (fstpp(x))) (interp (sndpp(x))); [auto|..].
 
   {
   elim (Hmemp1); intro HInp1; [apply HSS with s1|apply HSS with s2];
@@ -392,7 +432,7 @@ Lemma test_col_ok : forall ss sp interp p1 p2 p3,
 Proof.
 intros ss sp interp p1 p2 p3 HSS HSP HTC.
 unfold test_col in *.
-assert (HSS2 : ss_ok (identify_lines ss sp) interp)
+assert (HSS2 : ss_ok (identify_lines ss sp (cardinal ss)) interp)
   by (apply identify_lines_ok; assumption).
 unfold ss_ok in HSS2.
 apply exists_2 in HTC;
